rustdemo/HashMapLink.v
@@ -11,6 +11,7 @@ Require Import Invariant Smallstep SmallstepLinkingSafe.
 Require Import LinkedList HashMap.
 Require Import HashMapCommon LinkedListSafe HashMapSafe.
 Require Import MoveCheckingDomain.
+Require Import Rusttypes.
 Require Import InvariantAlgebra Compiler.
 
 Local Open Scope error_monad_scope.
@@ -18,62 +19,275 @@ Local Open Scope inv_scope.
 Import ListNotations.
 
 (* The linked_list module (implemented in Rustlight) is totally safe
-after the compilation *)
+after the compilation. The safety interface for the compiled module is
+
+⟦list.s⟧ ⊩ {process ↦ ⊤, hmap_process ↦ ⊥} ⋅ I_rs⋅R_ra
+        ↠ {find_process ↦ ⊤, hash ↦ P} ⋅ I_rs⋅R_ra
+ *)
 Lemma compiled_linked_list_safe: forall linked_list_asm,
   transf_rustlight_program linked_list_mod = OK linked_list_asm ->
-  module_type_safe ((hmap_inv @@ rs_own) @! cc_rust_compcert) ((hmap_inv @@ rs_own) @! cc_rust_compcert) (Asm.semantics linked_list_asm) SIF.
+  module_type_safe ((list_ext_inv @@ rs_own) @! cc_rust_compcert) ((hmap_ext_inv @@ rs_own) @! cc_rust_compcert) (Asm.semantics linked_list_asm) SIF.
 Proof.
   intros.
   eapply transf_rustlight_partial_safe_to_total_safe; eauto.
   eapply linked_list_module_safe.
 Qed.
 
-(* The hash_map module is totally safe after the compilation *)
+Definition hmap_size : nat := 10%nat.
+
+(* The hash_map module is totally safe after the compilation.
+
+⟦hmap.s⟧ ⊩ {find_process ↦ ⊤, hash ↦ P} ⋅ I_rs⋅R_rc⋅R_ca
+             ↠ {process ↦ ⊤⋅I_rs⋅R_rc, hmap_process ↦ Q} ⋅ R_ca
+ *)
 Lemma compiled_hash_map_safe: forall hash_map_asm,
   transf_clight_program hash_map_prog = OK hash_map_asm ->
-  module_type_safe ((hmap_inv @@ rs_own) @! cc_rust_compcert) ((hmap_inv @@ rs_own) @! cc_rust_compcert) (Asm.semantics hash_map_asm) SIF.
+  module_type_safe
+    (((hmap_ext_inv @@ rs_own) @! cc_rust_c) @! cc_compcert)
+    ((hmap_int_inv hmap_size) @! cc_compcert)
+    (Asm.semantics hash_map_asm) SIF.
 Proof.
   intros.
-  eapply open_safety_inv_ref.
-  3: { eapply transf_clight_total_safety_preservation. eauto.
-       eapply hash_map_module_safe. }
-  rewrite invcc_compose_assoc.
-  eapply cc_inv_ref. reflexivity.
-  eapply cc_rust_compcert_eqv.
-  red.
-  rewrite invcc_compose_assoc.
-  eapply cc_inv_ref. reflexivity.
-  eapply cc_rust_compcert_eqv.
+  eapply transf_clight_total_safety_preservation. eauto.
+  eapply hash_map_module_safe.
 Qed.
 
+(*   eapply open_safety_inv_ref. *)
+(*   3: { eapply transf_clight_total_safety_preservation. eauto. *)
+(*        eapply hash_map_module_safe. } *)
+(*   rewrite invcc_compose_assoc. *)
+(*   eapply cc_inv_ref. reflexivity. *)
+(*   eapply cc_rust_compcert_eqv. *)
+(*   red. *)
+(*   rewrite invcc_compose_assoc. *)
+(*   eapply cc_inv_ref. reflexivity. *)
+(*   eapply cc_rust_compcert_eqv. *)
+(* Qed. *)
+
 (** The syntactic linked assembly module (linked_list_asm +
-hash_map_asm) is totally safe under the invariant ((hmap_inv @@
-rs_own) @! cc_rust_compcert). *)
+hash_map_asm) is totally safe with the following safety interfaces.
+
+ ⟦hmap.s + list.s⟧ ⊩ ({find_process ↦ ⊤⋅I_rs⋅R_rc, hash ↦ P⋅I_rs⋅R_rc}
+                    ⊎ {process ↦ ⊤⋅I_rs⋅R_rc, hmap_process ↦ Q}) ⋅ R_ca
+                    ↠ 
+                    ({find_process ↦ ⊤⋅I_rs⋅R_rc, hash ↦ P⋅I_rs⋅R_rc}
+                    ⊎ {process ↦ ⊤⋅I_rs⋅R_rc, hmap_process ↦ Q}) ⋅ R_ca
+
+We want to separate the hmap_process from functions those have rust
+interfaces.
+
+ ⟦hmap.s + list.s⟧ ⊩ {find_process ↦ ⊤, hash ↦ P, process ↦ ⊤} ⋅I_rs⋅R_ra
+                     ⊎ {hmap_process ↦ Q}⋅ R_ca
+                     ↠ 
+                     {find_process ↦ ⊤, hash ↦ P, process ↦ ⊤} ⋅I_rs⋅R_ra
+                     ⊎ {hmap_process ↦ Q}⋅ R_ca
+
+ *)
+
+(* {find_process ↦ ⊤, hash ↦ P, process ↦ ⊤}. *)
+Definition hmap_rs_cond :=
+  hmap_ext_inv ⊎ list_ext_inv.
+
+(* {hmap_process ↦ Q} *)
+Definition cq_hmap_process N (w: hmap_world_int) (q: c_query) (fid: ident) : Prop :=
+  if ident_eq fid hmap_process then
+    vq_hmap_process N w q
+  else False.
+
+Definition cr_hmap_process N (w: hmap_world_int) (r: c_reply) (fid: ident) : Prop :=
+  if ident_eq fid hmap_process then
+    vr_hmap_process N w r
+  else False.
+
+
+(* {hmap_process ↦ Q} *)
+Definition hmap_process_cond N : invariant li_c :=
+  {| inv_world := hmap_world_int;
+    symtbl_inv w se := (list_senv_ext (hmap_list_ext w)) = se
+                       (* wf_xx_senv is used to ensure the safety of
+                       function call (see eval_Eglobal) *)
+                       /\ wf_senv se;
+    query_inv w q := cq_inv w q (list_senv_ext (hmap_list_ext w)) (cq_hmap_process N);
+    reply_inv w r := cr_inv w r (list_callee_ext (hmap_list_ext w)) (cr_hmap_process N)|}.
+
+
+Lemma invcc_id1 {liA: language_interface} (P: invariant liA):
+    invref (P@!1) P.
+Proof.
+  red. intros. destruct w1. inv H. inv H1. inv H0. inv H1.
+  inv H2. inv H3. 
+  exists i. repeat apply conj; auto.
+  intros. simpl.
+  exists r. split; auto.
+Qed.
+
+Lemma invcc_id2 {liA: language_interface} (P: invariant liA):
+    invref P (P@!1).
+Proof.
+  red. intros. exists (w1, tt).
+  repeat apply conj; try simpl; auto.
+  exists se. auto. exists q. eauto.
+  intros. destruct H1. destruct H1. subst. auto.
+Qed.
+
+
+Lemma module_type_safe_compose_id {liA liB: language_interface} P Q (L: semantics liA liB):
+      module_type_safe (P @! 1) (Q @! 1) L SIF ->
+      module_type_safe P Q L SIF.
+Proof.
+  intros.
+  eapply open_safety_inv_ref; eauto.
+  eapply invcc_id1. eapply invcc_id2.
+Qed.
+
+
+Lemma hmap_ext_inv_hmap_fun_disjoint: forall w vf sg args m,
+    query_inv hmap_ext_inv w (rsq vf sg args m) ->
+    Genv.is_internal (Genv.globalenv (hmap_senv_ext w) (Ctypes.program_of_program hash_map_prog)) vf = false.
+Proof.
+  intros. destruct w. simpl in H. red in H. simpl in H.
+  destruct vf; try contradiction.
+  destruct Ptrofs.eq_dec in H; try contradiction. subst.
+  destruct Genv.invert_symbol eqn: SYM in H; try contradiction.
+  red in H.
+  unfold Genv.is_internal, Genv.find_funct, Genv.find_funct_ptr.
+  rewrite dec_eq_true. rewrite Genv.find_def_spec. setoid_rewrite SYM.
+  repeat destruct ident_eq in H; try contradiction; subst; reflexivity.
+Qed.
+
+
 Theorem link_linked_list_hash_map_safe: forall linked_list_asm hash_map_asm linked_mod,
     transf_rustlight_program linked_list_mod = OK linked_list_asm ->
     transf_clight_program hash_map_prog = OK hash_map_asm ->
-    Linking.link linked_list_asm hash_map_asm = Some linked_mod ->
-    module_type_safe ((hmap_inv @@ rs_own) @! cc_rust_compcert) ((hmap_inv @@ rs_own) @! cc_rust_compcert) (Asm.semantics linked_mod) SIF.
+    Linking.link hash_map_asm linked_list_asm = Some linked_mod ->
+    module_type_safe
+      (* {find_process ↦ ⊤, hash ↦ P, process ↦ ⊤} ⋅I_rs⋅R_ra *)
+      (((hmap_rs_cond @@ rs_own) @! cc_rust_compcert)
+         (* ⊎ {hmap_process ↦ Q}⋅ R_ca *)
+         ⊎ (hmap_process_cond hmap_size @! cc_compcert))
+      (* The same as above *)
+      (((hmap_rs_cond @@ rs_own) @! cc_rust_compcert) ⊎ (hmap_process_cond hmap_size @! cc_compcert))
+      (Asm.semantics linked_mod) SIF.
 Proof.
   intros.
-  assert (SAFE: module_type_safe (((hmap_inv @@ rs_own) @! cc_rust_compcert) @! 1)
-                  (((hmap_inv @@ rs_own) @! cc_rust_compcert) @! 1) (Asm.semantics linked_mod) SIF).
+  (* 1. safety preservation under syntactic linking *)
+  assert (SAFE: module_type_safe
+    ((((hmap_rs_cond @@ rs_own) @! cc_rust_compcert)
+     ⊎ hmap_process_cond hmap_size @! cc_compcert) @! 1)
+    ((((hmap_rs_cond @@ rs_own) @! cc_rust_compcert)
+       ⊎ hmap_process_cond hmap_size @! cc_compcert) @! 1)
+    (Asm.semantics linked_mod) SIF).
   { eapply module_type_safe_preservation.
     2: { eapply AsmLinking.asm_linking_backward. eauto. }
-    eapply compose_total_type_safety; eauto.
-    eapply compiled_linked_list_safe; eauto.
-    eapply compiled_hash_map_safe; eauto.
-    unfold SmallstepLinking.compose. simpl.
-    erewrite Linking.link_erase_program; eauto. simpl.
-    f_equal. f_equal.
-    apply Axioms.functional_extensionality. intros [|]; auto. }      
-  eapply open_safety_inv_ref.
-  eapply cc_inv_ref. reflexivity.
-  eapply CallconvAlgebra.cc_compose_id_right.
-  red. eapply cc_inv_ref. reflexivity.
-  eapply CallconvAlgebra.cc_compose_id_right.
-  eapply open_safety_inv_ref; eauto.
-  rewrite invcc_compose_assoc. reflexivity.
-  rewrite invcc_compose_assoc. reflexivity.
+    (* 2. refinement of safety interfaces *)
+    eapply open_safety_inv_ref.
+    (* 2.1 prove safety composition *)
+    3: {
+      (** TODO: the senv must be valid  *)
+            eapply compose_total_type_safety_general.
+         (* 2.1.1 safety of hmap.s *)
+         4: { eapply compiled_hash_map_safe. eauto. }
+         (* 2.1.2 safety of list.s. It requires refienment *)
+         4: { eapply open_safety_inv_ref.
+              3: { eapply compiled_linked_list_safe. eauto. }
+              admit. admit. }
+         (* 2.1.3 disjointness of the safety interfaces for composition *)
+         { intros w q se SINV VQ QINV. destruct w as ((w1 & w2) & w3 & w4).
+           destruct QINV as (?q & Q1 & Q2).
+           destruct SINV as (?se & S1 & S2).           
+           (* use fsim to rewrite the valid_query *)
+           exploit clight_semantic_preservation.
+           eapply transf_clight_program_match. eauto. intros ([FSIM] & [BSIM]).
+           erewrite fsim_match_valid_query. 3: eapply Q2.
+           2: { eapply FSIM. eauto. eauto.
+                erewrite fsim_skel; eauto.
+                eapply match_senv_valid_for; eauto. }
+           (* destruct query_inv to show that valid query is false *)
+           destruct w1 as (w1' & w1'').
+           destruct Q1 as (?q & (Q11 & Q12) & Q13).
+           destruct S1 as (?se & (S11 & S12) & S13).           
+           inv S13. inv S11.
+           inv Q13. simpl. 
+           eapply hmap_ext_inv_hmap_fun_disjoint. eauto. }
+         (* similar to 2.1.3 *)
+         { intros w q se SINV VQ QINV. destruct w as (w1 & w2).
+           destruct QINV as (?q & Q1 & Q2).
+           destruct SINV as (?se & S1 & S2).
+           (* use fsim to rewrite the valid_query *)
+           exploit rustlight_semantic_preservation.
+           eapply transf_rustlight_program_match. eauto.
+           intros (FSIM & BSIM).
+           eapply CallconvAlgebra.open_fsim_ccref in FSIM.
+           2: { eapply cc_rust_compcert_eqv. }
+           2: { eapply cc_rust_compcert_eqv. }
+           destruct FSIM as [FSIM].
+           (** Maybe we can just prove the valid_query by definition as
+           we cannot construct a rust query *)
+           simpl.
+           destruct w2 as ((se21 & w21) & (se22 & w22) & (se23 & w23) & w24).
+           destruct Q2 as (q21 & Q21 & q22 & Q22 & q23 & Q23 & Q24).
+           destruct S2 as (S21 & S22 & S23 & S24).
+           inv S21. inv S22. inv Q21. inv Q22.
+           destruct q.
+           (* simplify *)
+           unfold Genv.is_internal, Genv.find_funct, Genv.find_funct_ptr.
+           simpl. destruct (r Asm.PC) eqn: PC; auto.
+           destruct Ptrofs.eq_dec; auto. subst.
+           simpl in Q24. destruct q23. inv Q24.
+           generalize (H6 Asm.PC). intros PCINJ.
+           fsim_match_valid_query
+           (* rewrite match_stbls of the cc_asm injp *)
+           match_prog_rustlight
+           rewrite 
+                     
+           (* inversion of cc_c_asm_injp *)
+           inv Q23. 
+           
+
+           match_senv
+           erewrite fsim_match_valid_query
+           
+           simpl.
+           match_prog
+           erewrite Genv.is_internal_match_id
+           Genv.is_internal
+           valid_query
+           simpl. 
+           
+           erewrite fsim_match_valid_query. 
+           2: { eapply FSIM. instantiate (1 := se0). instantiate (1 := (se0, tt, w2)).
+                econstructor. reflexivity. eauto.                
+                erewrite fsim_skel; eauto.
+                eapply match_senv_valid_for; eauto. }
+           simpl. 
+           (* destruct query_inv to show that valid query is false *)
+           instantiate (1 := q0).
+           simpl in S1. destruct S1 as ( S11 & S12).
+           destruct Q1 as (?q & (Q11 & Q12) & Q13).
+           destruct S1 as (?se & (S11 & S12) & S13).           
+           inv S13. inv S11.
+           inv Q13. simpl. 
+           eapply hmap_ext_inv_hmap_fun_disjoint. eauto. }
+
+                          
+           
+
+           
+         (* external calls are not valid incoming call *)
+         intros. destruct i.
+         simpl. destruct s. inv H2.
+         unfold Genv.is_internal. simpl. rewrite H3. reflexivity.
+         (* 2.1.4 semantic compose *)
+         unfold SmallstepLinking.compose. simpl.
+         erewrite Linking.link_erase_program; eauto. simpl.
+         f_equal. f_equal.
+         apply Axioms.functional_extensionality. intros [|]; auto.  }
+    (* 2.2 refinement of invariant *)
+    admit.
+    (* 2.3 refinement of invariant *)
+    admit. }
+  (* 3. refienment of the interface of Lowering *)
+  eapply module_type_safe_compose_id.
+  eauto.
 Qed.
 
